Translation/Example.v
@@ -50,7 +50,7 @@ Proof.
       destruct (IHbl (ssnoc Γ0 (svass nAnon A))) as [z hz].
       * econstructor.
         -- assumption.
-        -- eexists. eassumption.
+        -- eassumption.
       * econstructor.
         -- eassumption.
         -- assumption.
@@ -108,7 +108,7 @@ Proof.
       destruct (@type_multiProd (B :: bl0) (ssnoc Γ0 (svass nAnon A))) as [z hz].
       * econstructor.
         -- assumption.
-        -- eexists. eassumption.
+        -- eassumption.
       * eapply wbtm_wfb. eassumption.
       * eapply type_Lambda.
         -- eassumption.
@@ -116,7 +116,7 @@ Proof.
         -- eapply IHbl.
            ++ econstructor.
               ** assumption.
-              ** eexists. eassumption.
+              ** eassumption.
            ++ assumption.
 Defined.
 
@@ -150,233 +150,226 @@ Proof.
   - econstructor.
     + eapply type_Sort. constructor.
     + econstructor.
-      * eapply type_Sort. constructor.
-        -- constructor.
-        -- eexists. repeat constructor.
+      * eapply type_Sort. 
+        repeat econstructor. 
       * econstructor.
         -- eapply type_Eq.
            ++ repeat constructor.
-              ** eexists. repeat constructor.
-              ** eexists. repeat constructor.
-                 eexists. repeat constructor.
+              ** repeat econstructor.
            ++ refine (type_Rel _ _ _ _ _).
-              ** repeat constructor.
-                 --- eexists. repeat constructor.
-                 --- eexists. repeat constructor.
-                     eexists. repeat constructor.
+              ** repeat econstructor.
               ** cbn. omega.
            ++ refine (type_Rel _ _ _ _ _).
-              ** repeat constructor.
-                 --- eexists. repeat constructor.
-                 --- eexists. repeat constructor.
-                     eexists. repeat constructor.
+              ** repeat econstructor.
               ** cbn. omega.
         -- econstructor.
            ++ refine (type_Rel _ _ _ _ _).
-              ** repeat constructor.
-                 --- eexists. repeat constructor.
-                 --- eexists. repeat constructor.
-                     eexists. repeat constructor.
-                 --- eexists. eapply type_Eq.
-                     +++ repeat constructor.
-                         *** eexists. repeat constructor.
-                         *** eexists. repeat constructor.
-                             eexists. repeat constructor.
-                     +++ refine (type_Rel _ _ _ _ _).
-                         *** repeat constructor.
-                             ---- eexists. repeat constructor.
-                             ---- eexists. repeat constructor.
-                                  eexists. repeat constructor.
-                         *** cbn. omega.
-                     +++ refine (type_Rel _ _ _ _ _).
-                         *** repeat constructor.
-                             ---- eexists. repeat constructor.
-                             ---- eexists. repeat constructor.
-                                  eexists. repeat constructor.
-                         *** cbn. omega.
+              ** repeat econstructor.
+                 (* --- eexists. repeat constructor. *)
+                 (* --- eexists. repeat constructor. *)
+                 (*     eexists. repeat constructor. *)
+                 (* --- eexists. eapply type_Eq. *)
+                 (*     +++ repeat constructor. *)
+                 (*         *** eexists. repeat constructor. *)
+                 (*         *** eexists. repeat constructor. *)
+                 (*             eexists. repeat constructor. *)
+                 (*     +++ refine (type_Rel _ _ _ _ _). *)
+                 (*         *** repeat constructor. *)
+                 (*             ---- eexists. repeat constructor. *)
+                 (*             ---- eexists. repeat constructor. *)
+                 (*                  eexists. repeat constructor. *)
+                 (*         *** cbn. omega. *)
+                 (*     +++ refine (type_Rel _ _ _ _ _). *)
+                 (*         *** repeat constructor. *)
+                 (*             ---- eexists. repeat constructor. *)
+                 (*             ---- eexists. repeat constructor. *)
+                 (*                  eexists. repeat constructor. *)
+                 (*         *** cbn. omega. *)
               ** cbn. omega.
            ++ econstructor.
               ** refine (type_Rel _ _ _ _ _).
-                 --- repeat constructor.
-                     +++ eexists. repeat constructor.
-                     +++ eexists. repeat constructor.
-                         eexists. repeat constructor.
-                     +++ eexists. repeat constructor.
-                         *** eexists. repeat constructor.
-                         *** eexists. repeat constructor.
-                             eexists. repeat constructor.
-                         *** refine (type_Rel _ _ _ _ _).
-                             ---- repeat constructor.
-                                  ++++ eexists. repeat constructor.
-                                  ++++ eexists. repeat constructor.
-                                       eexists. repeat constructor.
-                             ---- cbn. omega.
-                         *** refine (type_Rel _ _ _ _ _).
-                             ---- repeat constructor.
-                                  ++++ eexists. repeat constructor.
-                                  ++++ eexists. repeat constructor.
-                                       eexists. repeat constructor.
-                             ---- cbn. omega.
-                     +++ eexists. refine (type_Rel _ _ _ _ _).
-                         *** econstructor.
-                             ---- repeat constructor.
-                                  ++++ eexists. repeat constructor.
-                                  ++++ eexists. repeat constructor.
-                                       eexists. repeat constructor.
-                             ---- eexists. eapply type_Eq.
-                                  ++++ repeat constructor.
-                                       **** eexists. repeat constructor.
-                                       **** eexists. repeat constructor.
-                                            eexists. repeat constructor.
-                                  ++++ refine (type_Rel _ _ _ _ _).
-                                       **** repeat constructor.
-                                            ----- eexists. repeat constructor.
-                                            ----- eexists. repeat constructor.
-                                                  eexists. repeat constructor.
-                                       **** cbn. omega.
-                                  ++++ refine (type_Rel _ _ _ _ _).
-                                       **** repeat constructor.
-                                            ----- eexists. repeat constructor.
-                                            ----- eexists. repeat constructor.
-                                                  eexists. repeat constructor.
-                                       **** cbn. omega.
-                         *** cbn. omega.
+                 --- repeat econstructor.
+                     (* +++ eexists. repeat constructor. *)
+                     (* +++ eexists. repeat constructor. *)
+                     (*     eexists. repeat constructor. *)
+                     (* +++ eexists. repeat constructor. *)
+                     (*     *** eexists. repeat constructor. *)
+                     (*     *** eexists. repeat constructor. *)
+                     (*         eexists. repeat constructor. *)
+                     (*     *** refine (type_Rel _ _ _ _ _). *)
+                     (*         ---- repeat constructor. *)
+                     (*              ++++ eexists. repeat constructor. *)
+                     (*              ++++ eexists. repeat constructor. *)
+                     (*                   eexists. repeat constructor. *)
+                     (*         ---- cbn. omega. *)
+                     (*     *** refine (type_Rel _ _ _ _ _). *)
+                     (*         ---- repeat constructor. *)
+                     (*              ++++ eexists. repeat constructor. *)
+                     (*              ++++ eexists. repeat constructor. *)
+                     (*                   eexists. repeat constructor. *)
+                     (*         ---- cbn. omega. *)
+                     (* +++ eexists. refine (type_Rel _ _ _ _ _). *)
+                     (*     *** econstructor. *)
+                     (*         ---- repeat constructor. *)
+                     (*              ++++ eexists. repeat constructor. *)
+                     (*              ++++ eexists. repeat constructor. *)
+                     (*                   eexists. repeat constructor. *)
+                     (*         ---- eexists. eapply type_Eq. *)
+                     (*              ++++ repeat constructor. *)
+                     (*                   **** eexists. repeat constructor. *)
+                     (*                   **** eexists. repeat constructor. *)
+                     (*                        eexists. repeat constructor. *)
+                     (*              ++++ refine (type_Rel _ _ _ _ _). *)
+                     (*                   **** repeat constructor. *)
+                     (*                        ----- eexists. repeat constructor. *)
+                     (*                        ----- eexists. repeat constructor. *)
+                     (*                              eexists. repeat constructor. *)
+                     (*                   **** cbn. omega. *)
+                     (*              ++++ refine (type_Rel _ _ _ _ _). *)
+                     (*                   **** repeat constructor. *)
+                     (*                        ----- eexists. repeat constructor. *)
+                     (*                        ----- eexists. repeat constructor. *)
+                     (*                              eexists. repeat constructor. *)
+                     (*                   **** cbn. omega. *)
+                     (*     *** cbn. omega. *)
                  --- cbn. omega.
               ** eapply type_conv''.
                  --- refine (type_Rel _ _ _ _ _).
-                     +++ repeat constructor.
-                         *** eexists. repeat constructor.
-                         *** eexists. repeat constructor.
-                             eexists. repeat constructor.
-                         *** eexists. repeat constructor.
-                             ---- eexists. repeat constructor.
-                             ---- eexists. repeat constructor.
-                                  eexists. repeat constructor.
-                             ---- refine (type_Rel _ _ _ _ _).
-                                  ++++ repeat constructor.
-                                       **** eexists. repeat constructor.
-                                       **** eexists. repeat constructor.
-                                            eexists. repeat constructor.
-                                  ++++ cbn. omega.
-                             ---- refine (type_Rel _ _ _ _ _).
-                                  ++++ repeat constructor.
-                                       **** eexists. repeat constructor.
-                                       **** eexists. repeat constructor.
-                                            eexists. repeat constructor.
-                                  ++++ cbn. omega.
-                         *** eexists. refine (type_Rel _ _ _ _ _).
-                             ---- repeat constructor.
-                                  ++++ eexists. repeat constructor.
-                                  ++++ eexists. repeat constructor.
-                                       eexists. repeat constructor.
-                                  ++++ eexists. repeat constructor.
-                                       **** eexists. repeat constructor.
-                                       **** eexists. repeat constructor.
-                                            eexists. repeat constructor.
-                                       **** refine (type_Rel _ _ _ _ _).
-                                            ----- repeat constructor.
-                                            +++++ eexists. repeat constructor.
-                                            +++++ eexists. repeat constructor.
-                                                  eexists. repeat constructor.
-                                            ----- cbn. omega.
-                                       **** refine (type_Rel _ _ _ _ _).
-                                            ----- repeat constructor.
-                                            +++++ eexists. repeat constructor.
-                                            +++++ eexists. repeat constructor.
-                                                  eexists. repeat constructor.
-                                            ----- cbn. omega.
-                             ---- cbn. omega.
+                     +++ repeat econstructor.
+                         (* *** eexists. repeat constructor. *)
+                         (* *** eexists. repeat constructor. *)
+                         (*     eexists. repeat constructor. *)
+                         (* *** eexists. repeat constructor. *)
+                         (*     ---- eexists. repeat constructor. *)
+                         (*     ---- eexists. repeat constructor. *)
+                         (*          eexists. repeat constructor. *)
+                         (*     ---- refine (type_Rel _ _ _ _ _). *)
+                         (*          ++++ repeat constructor. *)
+                         (*               **** eexists. repeat constructor. *)
+                         (*               **** eexists. repeat constructor. *)
+                         (*                    eexists. repeat constructor. *)
+                         (*          ++++ cbn. omega. *)
+                         (*     ---- refine (type_Rel _ _ _ _ _). *)
+                         (*          ++++ repeat constructor. *)
+                         (*               **** eexists. repeat constructor. *)
+                         (*               **** eexists. repeat constructor. *)
+                         (*                    eexists. repeat constructor. *)
+                         (*          ++++ cbn. omega. *)
+                         (* *** eexists. refine (type_Rel _ _ _ _ _). *)
+                         (*     ---- repeat constructor. *)
+                         (*          ++++ eexists. repeat constructor. *)
+                         (*          ++++ eexists. repeat constructor. *)
+                         (*               eexists. repeat constructor. *)
+                         (*          ++++ eexists. repeat constructor. *)
+                         (*               **** eexists. repeat constructor. *)
+                         (*               **** eexists. repeat constructor. *)
+                         (*                    eexists. repeat constructor. *)
+                         (*               **** refine (type_Rel _ _ _ _ _). *)
+                         (*                    ----- repeat constructor. *)
+                         (*                    +++++ eexists. repeat constructor. *)
+                         (*                    +++++ eexists. repeat constructor. *)
+                         (*                          eexists. repeat constructor. *)
+                         (*                    ----- cbn. omega. *)
+                         (*               **** refine (type_Rel _ _ _ _ _). *)
+                         (*                    ----- repeat constructor. *)
+                         (*                    +++++ eexists. repeat constructor. *)
+                         (*                    +++++ eexists. repeat constructor. *)
+                         (*                          eexists. repeat constructor. *)
+                         (*                    ----- cbn. omega. *)
+                         (*     ---- cbn. omega. *)
                      +++ cbn. omega.
                  --- cbn. eapply reflection.
                      instantiate (2 := sRel 1).
                      refine (type_Rel _ _ _ _ _).
-                     +++ repeat constructor.
-                         *** eexists. repeat constructor.
-                         *** eexists. repeat constructor.
-                             eexists. repeat constructor.
-                         *** eexists. repeat constructor.
-                             ---- eexists. repeat constructor.
-                             ---- eexists. repeat constructor.
-                                  eexists. repeat constructor.
-                             ---- refine (type_Rel _ _ _ _ _).
-                                  ++++ repeat constructor.
-                                       **** eexists. repeat constructor.
-                                       **** eexists. repeat constructor.
-                                            eexists. repeat constructor.
-                                  ++++ cbn. omega.
-                             ---- refine (type_Rel _ _ _ _ _).
-                                  ++++ repeat constructor.
-                                       **** eexists. repeat constructor.
-                                       **** eexists. repeat constructor.
-                                            eexists. repeat constructor.
-                                  ++++ cbn. omega.
-                         *** eexists. refine (type_Rel _ _ _ _ _).
-                             ---- repeat constructor.
-                                  ++++ eexists. repeat constructor.
-                                  ++++ eexists. repeat constructor.
-                                       eexists. repeat constructor.
-                                  ++++ eexists. repeat constructor.
-                                       **** eexists. repeat constructor.
-                                       **** eexists. repeat constructor.
-                                            eexists. repeat constructor.
-                                       **** refine (type_Rel _ _ _ _ _).
-                                            ----- repeat constructor.
-                                            +++++ eexists. repeat constructor.
-                                            +++++ eexists. repeat constructor.
-                                                  eexists. repeat constructor.
-                                            ----- cbn. omega.
-                                       **** refine (type_Rel _ _ _ _ _).
-                                            ----- repeat constructor.
-                                            +++++ eexists. repeat constructor.
-                                            +++++ eexists. repeat constructor.
-                                                  eexists. repeat constructor.
-                                            ----- cbn. omega.
-                             ---- cbn. omega.
+                     +++ repeat econstructor.
+                         (* *** eexists. repeat constructor. *)
+                         (* *** eexists. repeat constructor. *)
+                         (*     eexists. repeat constructor. *)
+                         (* *** eexists. repeat constructor. *)
+                         (*     ---- eexists. repeat constructor. *)
+                         (*     ---- eexists. repeat constructor. *)
+                         (*          eexists. repeat constructor. *)
+                         (*     ---- refine (type_Rel _ _ _ _ _). *)
+                         (*          ++++ repeat constructor. *)
+                         (*               **** eexists. repeat constructor. *)
+                         (*               **** eexists. repeat constructor. *)
+                         (*                    eexists. repeat constructor. *)
+                         (*          ++++ cbn. omega. *)
+                         (*     ---- refine (type_Rel _ _ _ _ _). *)
+                         (*          ++++ repeat constructor. *)
+                         (*               **** eexists. repeat constructor. *)
+                         (*               **** eexists. repeat constructor. *)
+                         (*                    eexists. repeat constructor. *)
+                         (*          ++++ cbn. omega. *)
+                         (* *** eexists. refine (type_Rel _ _ _ _ _). *)
+                         (*     ---- repeat constructor. *)
+                         (*          ++++ eexists. repeat constructor. *)
+                         (*          ++++ eexists. repeat constructor. *)
+                         (*               eexists. repeat constructor. *)
+                         (*          ++++ eexists. repeat constructor. *)
+                         (*               **** eexists. repeat constructor. *)
+                         (*               **** eexists. repeat constructor. *)
+                         (*                    eexists. repeat constructor. *)
+                         (*               **** refine (type_Rel _ _ _ _ _). *)
+                         (*                    ----- repeat constructor. *)
+                         (*                    +++++ eexists. repeat constructor. *)
+                         (*                    +++++ eexists. repeat constructor. *)
+                         (*                          eexists. repeat constructor. *)
+                         (*                    ----- cbn. omega. *)
+                         (*               **** refine (type_Rel _ _ _ _ _). *)
+                         (*                    ----- repeat constructor. *)
+                         (*                    +++++ eexists. repeat constructor. *)
+                         (*                    +++++ eexists. repeat constructor. *)
+                         (*                          eexists. repeat constructor. *)
+                         (*                    ----- cbn. omega. *)
+                         (*     ---- cbn. omega. *)
                      +++ cbn. omega.
                  --- refine (type_Rel _ _ _ _ _).
-                     +++ repeat constructor.
-                         *** eexists. repeat constructor.
-                         *** eexists. repeat constructor.
-                             eexists. repeat constructor.
-                         *** eexists. repeat constructor.
-                             ---- eexists. repeat constructor.
-                             ---- eexists. repeat constructor.
-                                  eexists. repeat constructor.
-                             ---- refine (type_Rel _ _ _ _ _).
-                                  ++++ repeat constructor.
-                                       **** eexists. repeat constructor.
-                                       **** eexists. repeat constructor.
-                                            eexists. repeat constructor.
-                                  ++++ cbn. omega.
-                             ---- refine (type_Rel _ _ _ _ _).
-                                  ++++ repeat constructor.
-                                       **** eexists. repeat constructor.
-                                       **** eexists. repeat constructor.
-                                            eexists. repeat constructor.
-                                  ++++ cbn. omega.
-                         *** eexists. refine (type_Rel _ _ _ _ _).
-                             ---- repeat constructor.
-                                  ++++ eexists. repeat constructor.
-                                  ++++ eexists. repeat constructor.
-                                       eexists. repeat constructor.
-                                  ++++ eexists. repeat constructor.
-                                       **** eexists. repeat constructor.
-                                       **** eexists. repeat constructor.
-                                            eexists. repeat constructor.
-                                       **** refine (type_Rel _ _ _ _ _).
-                                            ----- repeat constructor.
-                                            +++++ eexists. repeat constructor.
-                                            +++++ eexists. repeat constructor.
-                                                  eexists. repeat constructor.
-                                            ----- cbn. omega.
-                                       **** refine (type_Rel _ _ _ _ _).
-                                            ----- repeat constructor.
-                                            +++++ eexists. repeat constructor.
-                                            +++++ eexists. repeat constructor.
-                                                  eexists. repeat constructor.
-                                            ----- cbn. omega.
-                             ---- cbn. omega.
+                     +++ repeat econstructor.
+                         (* *** eexists. repeat constructor. *)
+                         (* *** eexists. repeat constructor. *)
+                         (*     eexists. repeat constructor. *)
+                         (* *** eexists. repeat constructor. *)
+                         (*     ---- eexists. repeat constructor. *)
+                         (*     ---- eexists. repeat constructor. *)
+                         (*          eexists. repeat constructor. *)
+                         (*     ---- refine (type_Rel _ _ _ _ _). *)
+                         (*          ++++ repeat constructor. *)
+                         (*               **** eexists. repeat constructor. *)
+                         (*               **** eexists. repeat constructor. *)
+                         (*                    eexists. repeat constructor. *)
+                         (*          ++++ cbn. omega. *)
+                         (*     ---- refine (type_Rel _ _ _ _ _). *)
+                         (*          ++++ repeat constructor. *)
+                         (*               **** eexists. repeat constructor. *)
+                         (*               **** eexists. repeat constructor. *)
+                         (*                    eexists. repeat constructor. *)
+                         (*          ++++ cbn. omega. *)
+                         (* *** eexists. refine (type_Rel _ _ _ _ _). *)
+                         (*     ---- repeat constructor. *)
+                         (*          ++++ eexists. repeat constructor. *)
+                         (*          ++++ eexists. repeat constructor. *)
+                         (*               eexists. repeat constructor. *)
+                         (*          ++++ eexists. repeat constructor. *)
+                         (*               **** eexists. repeat constructor. *)
+                         (*               **** eexists. repeat constructor. *)
+                         (*                    eexists. repeat constructor. *)
+                         (*               **** refine (type_Rel _ _ _ _ _). *)
+                         (*                    ----- repeat constructor. *)
+                         (*                    +++++ eexists. repeat constructor. *)
+                         (*                    +++++ eexists. repeat constructor. *)
+                         (*                          eexists. repeat constructor. *)
+                         (*                    ----- cbn. omega. *)
+                         (*               **** refine (type_Rel _ _ _ _ _). *)
+                         (*                    ----- repeat constructor. *)
+                         (*                    +++++ eexists. repeat constructor. *)
+                         (*                    +++++ eexists. repeat constructor. *)
+                         (*                          eexists. repeat constructor. *)
+                         (*                    ----- cbn. omega. *)
+                         (*     ---- cbn. omega. *)
                      +++ cbn. omega.
+                         Unshelve.
+                         all: cbn; omega. 
 Defined.
 
 (* Then we translate this ETT derivation to get an ITT term *)
@@ -388,6 +381,9 @@ Proof.
   - constructor.
   - constructor.
 Defined.
+
+Definition type_translation {Σ Γ t A} h {Γ'} hΓ :=
+  pi2_ _ _ (pi1_ _ _ (@complete_translation Σ)) Γ t A h Γ' hΓ.
 
 Definition itt_tm : sterm.
   destruct (type_translation tmty istrans_nil) as [A [t h]].
@@ -435,29 +431,19 @@ Proof.
   eapply type_multiLam.
   - constructor.
   - econstructor.
-    + repeat constructor.
+    + repeat econstructor.
     + econstructor.
       * refine (type_Rel _ _ _ _ _).
-        -- repeat constructor.
-           eexists. repeat constructor.
+        -- repeat econstructor.
         -- cbn. omega.
       * econstructor.
         -- refine (type_Rel _ _ _ _ _).
-           ++ repeat constructor.
-              ** eexists. repeat constructor.
-              ** eexists. refine (type_Rel _ _ _ _ _).
-                 --- repeat constructor.
-                     eexists. repeat constructor.
-                 --- cbn. omega.
+           ++ repeat econstructor.
            ++ cbn. omega.
         -- refine (type_Rel _ _ _ _ _).
-           ++ repeat constructor.
-              ** eexists. repeat constructor.
-              ** eexists. refine (type_Rel _ _ _ _ _).
-                 --- repeat constructor.
-                     eexists. repeat constructor.
-                 --- cbn. omega.
+           ++ repeat econstructor.
            ++ cbn. omega.
+  Unshelve. all: cbn; omega. 
 Defined.
 
 Definition itt_tm0 : sterm.
@@ -466,62 +452,10 @@ Definition itt_tm0 : sterm.
 Defined.
 
 (* Same problem with such a small example! *)
-(* Eval lazy in itt_tm0. *)
+Eval lazy in itt_tm0.
 
 Print Assumptions itt_tm0.
 Print Assumptions tmty0.
-
-(* Goal itt_tm0 = cheating. *)
-(* unfold itt_tm0. *)
-(* Opaque type_translation. *)
-(* cbn. Transparent type_translation. *)
-(* unfold type_translation. *)
-(* set (choose_type (A:= sSort (sType "Set+1")) (type_headSort (sType "Set+1")) *)
-(*          (let (i, _) := istrans_nil in i, inrel_Sort (succ_sort sSet), *)
-(*          inrel_Sort sSet, *)
-(*          ITyping.type_Sort Σ [] sSet (let (_, w0) := istrans_nil in w0))). *)
-(* Opaque choose_type. cbn in s. Transparent choose_type. unfold choose_type in s. *)
-(* unfold choose_type' in s. *)
-(* match goal with | s := let (_,_) := ?X in _ : _ |- _ => set X in * end. *)
-(* cbn in s0. unfold s0 in s. clear s0. *)
-(* match goal with | s := let (_,_) := ?X in _ : _ |- _ => set X in * end. *)
-(* cbn in s0. unfold s0 in s; clear s0. *)
-(* match goal with | s := let (_,_) := ?X in _ : _ |- _ => set X in * end. *)
-(* Opaque Σ. *)
-(* lazy in s0. unfold s0 in s; clear s0. *)
-
-(* unfold s; clear s. *)
-(* match goal with *)
-(* | |- context [ let (p,hp) := ?X in let (q, hq) := sort_heq_ex hp in _ ] => set X *)
-(* end. *)
-(* Opaque trel_to_heq. lazy in s. Transparent trel_to_heq. *)
-(* unfold trel_to_heq, trel_to_heq' in s. *)
-(* unfold trel_rec, trel_rect in s. unfold s; clear s. *)
-(* match goal with *)
-(* | |- context [ sort_heq_ex ?X  ] => set (sort_heq_ex X) *)
-(* end. *)
-(* Opaque sort_heq_ex. unfold type_conv'  in s. *)
-(* Opaque eq_typing. lazy in s. *)
-(* Transparent sort_heq_ex. unfold sort_heq_ex  in s. *)
-(* unfold s; clear s. *)
-(* match goal with *)
-(* | |-  context [f_equal ?X ?Y]  => set (f_equal X Y) *)
-(* end. *)
-(* lazy in e. unfold e; clear e. unfold eq_rec_r, eq_rec, eq_rect. *)
-(* Opaque choose_type. unfold eq_sym. *)
-(* match goal with *)
-(* | |-  context [let (A, s) := *)
-(*      let (S', s) := *)
-(*        let (T', p) := ?X in _ in _ in _]  => set X *)
-(* end. *)
-
-(*  unfold eq_sym. *)
-(* unfold trel_trans, trel_sym. unfold trel_rec, trel_rect. *)
-(* lazy. *)
-(* unfold s; clear s. *)
-(* assert (H = H). clear s. Focus 1. lazy in H. *)
-(* lazy in s. *)
-(* Abort. *)
 
 (* One more *)
 
